get byte count

UTF8.fst
@@ -1,6 +1,9 @@
-module UTF8
+module FStar.BytesUTF
 
 open FStar.Seq
+open FStar.Char
+//include FStar.List.Tot
+
 
 module U = FStar.UInt
 module U8 = FStar.UInt8
@@ -15,6 +18,14 @@ abstract type string = seq FStar.Char.char
 assume val utf8_encode: string -> bytes
 assume val utf8_decode: bytes -> option string
 
-let main =
-  IO.print_string ("UTF-8 Encoding");
-  ()
+(* UTF-8 Encoding *)
+val get_byte_count: s:string { length s >= 4 /\ length s <= 5}  -> Tot(nat)
+let get_byte_count s =
+  if length s = 5 then 4 else
+    let first = head s in
+      let second = head (tail s) in
+        let third = head (tail (tail s)) in
+          let fourth = last s in
+            if (int_of_char first = 48 && int_of_char second = 48 && int_of_char third < 55 ) then 1
+            else if (int_of_char first = 48 && int_of_char second >= 48 && int_of_char third <= 55 ) then 2
+            else 3
